\documentclass{article}
\usepackage[usenames]{color}
\usepackage{minted}
\usepackage[utf8]{inputenc}
\usepackage[T1]{fontenc}
\usepackage{graphicx}
\usepackage{grffile}
% Package longtable omitted
% Package wrapfig omitted
% Package rotating omitted
\usepackage[normalem]{ulem}
\usepackage{amsmath}
\usepackage{textcomp}
\usepackage{amssymb}
% Package capt-of omitted
% Package hyperref omitted
\pagestyle{empty}             % do not remove
% The settings below are copied from fullpage.sty
\setlength{\textwidth}{\paperwidth}
\addtolength{\textwidth}{-3cm}
\setlength{\oddsidemargin}{1.5cm}
\addtolength{\oddsidemargin}{-2.54cm}
\setlength{\evensidemargin}{\oddsidemargin}
\setlength{\textheight}{\paperheight}
\addtolength{\textheight}{-\headheight}
\addtolength{\textheight}{-\headsep}
\addtolength{\textheight}{-\footskip}
\addtolength{\textheight}{-3cm}
\setlength{\topmargin}{1.5cm}
\addtolength{\topmargin}{-2.54cm}

\addbibresource{../Resources/references.bib}

\begin{document}
\begin{align*}
a_0= 1 \\
a_0= 1 \\
a_{n+  2} =  a_{n+  1 +  2 a_n}, \quad n \geq 0
\end{align*}
$f(x)$
\begin{align}
f\left( x \right)= \sum^{\infty}_{n= 0}   \left[ a_nx^n \right] \label{eq:pow-gen-func-np0}
\end{align}
\begin{align}
    \sum^{\infty}_{n= 0}  \left[ a_{n+  1} x^n \right] &= \frac{f\left( x \right)- a_0}{x} \label{eq:pow-gen-func-np1} \\
\sum^{\infty}_{n= 0}  \left[ a_{n+  2} x^n \right]  &= \frac{f\left( x \right) - a_0 - a_1x}{x^2} \label{eq:pow-gen-func-np2}
\end{align}
\begin{align}
    2a_n +  a_{n+  1 }&= a_{n+  2} \nonumber \\
    2a_nx^n +  a_{n+  1 } x^n &= a_{n+  2} x^n \nonumber \\
    \sum^{\infty}_{n= 0}   \left[ 2a_nx^n \right] + \sum^{\infty}_{n= 0}   \left[  a_{n+  1 } x^n  \right]   &= \sum^{\infty}_{n= 0}   \left[ a_{n+  2} x^n   \right] \label{eq:series-rep-pow-example}
\end{align}
\begin{align}
2f\left( x \right) +  \frac{f\left( x \right)- a_0}{x} &= \frac{f\left( x \right)- a_0}{- a_1x}x^2 \nonumber \\
\implies  f\left( x \right) &=  \frac{1}{1- x- x^2} \label{eq:power-series-form-example}
\end{align}
$2$
\begin{align*}
    f\left( x \right)&= \frac{1}{1- x- x^2}\\
&= \frac{- 1}{x^2 +  x -  1}\\
&= \frac{- 1}{\left( x- 2 \right)\left( x- 1 \right)}\\
&= \frac{A_1}{x- 2}+  \frac{A_2}{x- 1}, \quad A_i \in \mathbb{R}, i \in \mathbb{Z}^+ \\
 \implies  - 1 &= A_1\left( x- 1 \right) +  A_2\left( x- 2 \right)\\
 \text{Let $x$ = 2:}\\
 - 1&= A_1\left( 2-1 \right) +  0 \\
&= A_1 = - 1 \\
 \text{Let $x$ = 1:}\\
 - 1 &=  0 +  A_2 \left( 1- 2 \right) \\
 \implies  A_2&= 1 \\
 \text{Hence:}\\
 f\left( x \right)&=    \frac{1}{x- 1} - \frac{1}{x- 2}
\end{align*}
$$\begin{align*}
\sum^{\infty}_{n= 0}\left[ rx^n \right] = \frac{1}{1- rx^n}
\end{align*}$$
$$\begin{align*}
\frac{1}{x- 1}&= -\frac{1}{1 -\left( 1 \right) x} \\
&= -\sum^{\infty}_{n= 0}\left[ x^n \right]  \\
\frac{-1}{x- 2} &= \frac{1}{2- x} \\
&= \frac{1}{2}\frac{1}{1-\frac{1}{2}x} \\
&= \frac{1}{2} \sum^{\infty}_{n= 0}\left[ \left( \frac{1}{2}x \right) ^n \right]
\end{align*}$$
$$\begin{align*}
f\left( x \right) &= \frac{1}{2}\sum^{\infty}_{n= 0}\left[ \left( \frac{1}{2}x \right) ^n \right] - \sum^{\infty}_{n= 0}\left[ x^n \right] \\
f\left( x \right) &= \sum^{\infty}_{n= 0}\left[ \frac{1}{2}\left( \frac{1}{2}x \right) ^n -x^n \right]  \\
f\left( x \right) &= \sum^{\infty}_{n= 0}\left[ \frac{1}{2 \cdot 2^n} x^n -x^n \right]  \\
f\left( x \right) &= \sum^{\infty}_{n= 0}\left[x^n {\left( {\frac{1}{2 \cdot 2^n} -1} \right) } \right]  \\
 \implies  a_n &= \frac{1}{2 \cdot 2^n} - 1
\end{align*}$$
$a_n$
$\sum^\infty_{n = 0} \left[ a_nx^n \right]$
\begin{align*}
    a_{n}&= a_{n - 1} + a_{n - 2}\\
\iff a_{n+  2} &= a_{n+  1} +  a_n
\end{align*}
\begin{align*}
x^2 f\left( x \right) -  x f \left( x \right) -  f\left( x \right)=  0
\end{align*}
\begin{align*}
f''\left( x \right)- f'\left( x \right)- f\left( x \right)=  0
\end{align*}
$f\left( x \right)= e^x$
$\frac{\mathrm{d}\left( e^x \right) }{\mathrm{d} x} = e^x$
\begin{align*}
f\left( x \right)= e^rx = \sum^{\infty}_{n= 0}   \left[ r \frac{x^n}{n!} \right]
\end{align*}
$f(x)=e^x$
\begin{align*}
    f\left( x \right) &=  \sum^{\infty}_{n= 0}   \left[ a_{n} \cdot  \frac{x^n}{n!} \right]   &= e^x \\
    \text{ $\mathcal{TODO::}$ The real trick is showing this derivative property } \\
    f'\left( x \right) &=  \sum^{\infty}_{n= 0}   \left[ a_{n+1} \cdot  \frac{x^n}{n!} \right]  &= e^x \\
    f''\left( x \right) &=  \sum^{\infty}_{n= 0}   \left[ a_{n+2} \cdot  \frac{x^n}{n!} \right] &= e^x \\
\end{align*}
\begin{align*}
a_{n+  2}    &= a_{n+  1} +  a_{n}\\
\frac{x^n}{n!}   a_{n+  2}    &= \frac{x^n}{n!}\left( a_{n+  1} +  a_{n}  \right)\\
\sum^{\infty}_{n= 0} \left[ \frac{x^n}{n!}   a_{n+  2} \right]        &= \sum^{\infty}_{n= 0}   \left[ \frac{x^n}{n!} a_{n+  1} \right]  + \sum^{\infty}_{n= 0}   \left[ \frac{x^n}{n!} a_{n}  \right]  \\
f''\left( x \right) &= f'\left( x \right)+  f\left( x \right)
\end{align*}
\begin{align*}
f\left( x \right)= c_1 \cdot  \mathrm{exp}\left[ \left( \frac{1- \sqrt{5} }{2} \right)x \right] +  c_2 \cdot  \mathrm{exp}\left[ \left( \frac{1 +  \sqrt{5} }{2} \right) \right]
\end{align*}
\begin{align*}
f\left( x \right)&= \sum^{\infty}_{n= 0}   \left[ \left( c_1\left( \frac{1- \sqrt{5} }{2} \right)^n +  c_2 \cdot  \left( \frac{1+ \sqrt{5} }{2} \right)^n \right) \cdot  \frac{x^n}{n} \right]
\end{align*}
\begin{align*}
f\left( x \right)= \sum^{\infty}_{n= 0}   \left[ a_n \frac{x^n}{n!} \right]
\end{align*}
\begin{align*}
a_n = c_1\cdot  \left( \frac{1- \sqrt{5} }{2} \right)^n +  c_2 \cdot  \left( \frac{1+  \sqrt{5} }{2} \right)
\end{align*}
\begin{align*}
a_0= c_1 +  c_2  \implies  c_1= - c_2\\
a_1= c_1 \left( \frac{1+ \sqrt{5} }{2} \right) -  c_1 \frac{1-\sqrt{5} }{2}  \implies  c_1 = \frac{1}{\sqrt{5} }
\end{align*}
\begin{align*}
    a_n &= \frac{1}{\sqrt{5} } \left[ \left( \frac{1+  \sqrt{5} }{2}  \right)^n -  \left( \frac{1- \sqrt{5} }{2} \right)^n \right] \\
&= \frac{\varphi^n - \psi^n}{\sqrt{5} } \\
&= \frac{\varphi^n -  \psi^n}{\varphi - \psi}
\end{align*}
$\varphi = \frac{1+ \sqrt{5} }{2} \approx 1.61\ldots$
$\psi = 1-\varphi = \frac{1- \sqrt{5} }{2} \approx 0.61\ldots$
$a_{n+ 2}$
\end{document}
%%Local Variables:
%%TeX-master: t
%%End:
